feat(*) tidy optimised compiler

HOL_To_IMP-/HOL_Nat_To_IMP-/Compile_HOL_Nat_To_IMP/Compile_HOL_Nat_To_IMP.thy
@@ -5,8 +5,9 @@ theory Compile_HOL_Nat_To_IMP
     IMP_Terminates_With
     HOL_Nat_To_IMP_Minus_Base
     HOL_To_HOL_Nat.HOL_To_HOL_Nat_Basics
+    "HOL-Library.AList"
   keywords
-    "compile_nat" :: thy_decl and "compile_nat_old" :: thy_decl and "basename" and
+    "compile_nat" :: thy_decl and "basename" and "non-optimized" and
     "declare_compiled_const" :: thy_decl and
     "return_register" and "argument_registers" and "compiled" and
     "print_compiled_consts" :: diag
@@ -127,19 +128,13 @@ lemma tbig_step_pull_tIf_iff:
   by (induction c arbitrary: s t s' rule: pull_tIf_assoc_right.induct)
   (fastforce simp: tbig_step_t_assoc_right_tSeq tbig_step_pull_tIf_iff_aux)+
 
-fun al_get :: "vname \<Rightarrow> (vname \<times> atomExp) list \<Rightarrow> atomExp" where
-  "al_get x ((a,b)#ys) = (if x = a then b else al_get x ys)"
-| "al_get x [] = V x"
+definition "get_reg al r \<equiv> case map_of al r of None \<Rightarrow> V r | Some x \<Rightarrow> x"
 
-fun al_set :: "vname \<Rightarrow> atomExp \<Rightarrow> (vname \<times> atomExp) list \<Rightarrow> (vname \<times> atomExp) list" where
-  "al_set a b ((a',b')#xs) = (if a = a' then (a',b)#xs else (a',b') # al_set a b xs)"
-| "al_set a b [] = [(a,b)]"
-
-lemma al_get_al_set: "al_get x (al_set x y al) = y"
-  by (induction al) auto
+lemma get_reg_upadte_eq: "get_reg (AList.update x y al) x = y"
+  unfolding get_reg_def by (induction al) auto
 
 fun subst_atomExp :: "atomExp \<Rightarrow> (vname \<times> atomExp) list \<Rightarrow> atomExp" where
-  "subst_atomExp (V var) al = al_get var al"
+  "subst_atomExp (V r) al = get_reg al r"
 | "subst_atomExp a _ = a"
 
 fun subst_aexp :: "aexp \<Rightarrow> (vname \<times> atomExp) list \<Rightarrow> aexp" where
@@ -147,42 +142,49 @@ fun subst_aexp :: "aexp \<Rightarrow> (vname \<times> atomExp) list \<Rightarrow
 | "subst_aexp (Plus a1 a2) al = Plus (subst_atomExp a1 al) (subst_atomExp a2 al)"
 | "subst_aexp (Sub a1 a2) al = Sub (subst_atomExp a1 al) (subst_atomExp a2 al)"
 
-lemma tbig_step_subst_aexp_iff_if_aval_eq:
-  includes tcom_syntax
-  assumes "aval (subst_aexp a al) s = aval a s"
-  shows "C \<turnstile> (v ::= (subst_aexp a al), s) \<Rightarrow>\<^bsup>t\<^esup> s' \<longleftrightarrow> C \<turnstile> (v ::= a, s) \<Rightarrow>\<^bsup>t\<^esup> s'"
-  by (metis assms tAssign tAssign_tE)
+fun trans_assigns_aux :: "tcom \<Rightarrow> (vname \<times> atomExp) list \<Rightarrow> tcom \<times> (vname \<times> atomExp) list" where
+  "trans_assigns_aux (tSeq c1 c2) al = (
+    let
+      (c1', al') = trans_assigns_aux c1 al;
+      (c2', al'') = trans_assigns_aux c2 al'
+    in (tSeq c1' c2', al''))"
+| "trans_assigns_aux (tIf v c1 c2) al = (
+    let
+      (c1', al'1) = trans_assigns_aux c1 al;
+      (c2', al'2) = trans_assigns_aux c2 al
+    in (tIf (case get_reg al v of (V v') \<Rightarrow> v' | _ \<Rightarrow> v) c1' c2', filter (List.member al'2) al'1))"
+| "trans_assigns_aux (tAssign v a) al = (let a' = subst_aexp a al
+    in (tAssign v a', case a' of A atom \<Rightarrow> AList.update v atom al | _ \<Rightarrow> al))"
+| "trans_assigns_aux (tCall c v) al = (tCall c v, filter (\<lambda>(_, v'). v' \<noteq> V v) al)"
+| "trans_assigns_aux c al = (c, al)"
 
-fun ListMem' where
-  "ListMem' [] _ = False"
-| "ListMem' (x#xs) y = (x = y \<or> ListMem' xs y)"
+definition "trans_assigns c \<equiv> fst (trans_assigns_aux c [])"
 
-fun trans_assns_aux ::
-    "tcom \<Rightarrow> (vname \<times> atomExp) list \<Rightarrow> tcom \<times> (vname \<times> atomExp) list" where
-  "trans_assns_aux (tSeq c1 c2) al = (let (c1', al') = trans_assns_aux c1 al;
-    (c2', al'') = trans_assns_aux c2 al' in (tSeq c1' c2', al''))"
-| "trans_assns_aux (tIf v c1 c2) al =
-    (let (c1', al'1) = trans_assns_aux c1 al; (c2', al'2) = trans_assns_aux c2 al in
-    (tIf (case al_get v al of (V v') \<Rightarrow> v' | _ \<Rightarrow> v) c1' c2', filter (ListMem' al'2) al'1))"
-| "trans_assns_aux (tAssign v a) al = (let a' = subst_aexp a al in
-    (tAssign v a', (case a' of A atom \<Rightarrow> al_set v atom al | _ \<Rightarrow> al)))"
-| "trans_assns_aux (tCall c v) al = (tCall c v, filter (\<lambda>(_, v'). v' \<noteq> V v) al)"
-| "trans_assns_aux c al = (c, al)"
-definition "trans_assns c \<equiv> fst (trans_assns_aux c [])"
+definition "register_sep \<equiv> ''.''"
+definition "arg_sep \<equiv> ''arg''"
+definition "is_prefix xs ys \<equiv> take (length ys) xs = ys"
 
 fun is_arg :: "vname \<Rightarrow> bool" where
-  "is_arg (x#xs) = (take 6 xs = ''.args.'' \<or> is_arg xs)"
+  "is_arg (x # xs) = (is_prefix xs (register_sep @ arg_sep @ register_sep) \<or> is_arg xs)"
 | "is_arg [] = False"
 
 fun bury_aux :: "tcom \<Rightarrow> vname list \<Rightarrow> tcom \<times> vname list" where
-  "bury_aux (tSeq c1 c2) vl = (let (c2', vl') = bury_aux c2 vl;
-    (c1', vl'') = bury_aux c1 vl' in (tSeq c1' c2', vl''))"
-| "bury_aux (tIf v c1 c2) vl = (let (c1', vl'1) = bury_aux c1 vl;
-    (c2', vl'2) = bury_aux c2 vl in (tIf v c1' c2', v # vl'1 @ vl'2))"
-| "bury_aux (tAssign v a) vl = (if a = A (V v) \<or> \<not>(ListMem' vl v \<or> is_arg v)
-    then (tSKIP, vl) else (tAssign v a, vars a @ (filter (\<lambda>x. x \<noteq> v) vl)))"
-| "bury_aux (tCall c v) vl = (if ListMem' vl v then
-    (tCall c v, filter (\<lambda>x. x \<noteq> v) vl) else (tSKIP, vl))"
+  "bury_aux (tSeq c1 c2) vl = (
+    let
+      (c2', vl') = bury_aux c2 vl;
+      (c1', vl'') = bury_aux c1 vl'
+    in (tSeq c1' c2', vl''))"
+| "bury_aux (tIf v c1 c2) vl = (
+    let
+      (c1', vl'1) = bury_aux c1 vl;
+      (c2', vl'2) = bury_aux c2 vl
+    in (tIf v c1' c2', v # vl'1 @ vl'2))"
+| "bury_aux (tAssign v a) vl = (if a = A (V v) \<or> (v \<notin> set vl \<and> \<not>is_arg v)
+    then (tSKIP, vl)
+    else (tAssign v a, vars a @ filter ((\<noteq>) v) vl))"
+| "bury_aux (tCall c v) vl = (if v \<in> set vl
+    then (tCall c v, filter ((\<noteq>) v) vl)
+    else (tSKIP, vl))"
 | "bury_aux c vl = (c, vl)"
 definition
   "bury ret_reg c \<equiv> fst (bury_aux c [ret_reg])"
@@ -202,4 +204,5 @@ end
 declare tailcall_to_IMP_Minus_def[code del]
 
 ML_file\<open>compile_hol_nat_to_imp.ML\<close>
+
 end
